src/Interval.v
@@ -1,6 +1,7 @@
 Require Import LinearScan.Lib.
 Require Import LinearScan.Range.
 Require Import LinearScan.UsePos.
+Require Import Coq.Strings.String.
 
 Set Implicit Arguments.
 Unset Strict Implicit.
