src/Ssr.v
@@ -1,0 +1,22 @@
+From Coq Require Export ssreflect ssrfun ssrbool.
+From mathcomp Require Export eqtype seq ssrnat fintype.
+
+Lemma and_swap : forall x y z, [&& x, y & z] = [&& y, x & z].
+Proof. by case; case; case. Qed.
+
+Definition decide {T : Type} (H : bool)
+  (kt : (H = true)  -> T)
+  (kf : (H = false) -> T) : T :=
+  (fun (if_true  : (fun b : bool => protect_term (H = b) -> T) true)
+       (if_false : (fun b : bool => protect_term (H = b) -> T) false) =>
+    if H as b return ((fun b0 : bool => protect_term (H = b0) -> T) b)
+    then if_true
+    else if_false)
+  (fun (E : H = true)  => kt E)
+  (fun (E : H = false) => kf E)
+  (erefl H).
+
+Arguments decide {T} H kt kf.
+
+Definition prop (b : bool) : option (is_true b) :=
+  if b then Some is_true_true else None.
