default.nix
@@ -1,0 +1,76 @@
+args@{
+  rev    ? "9222ae36b208d1c6b55d88e10aa68f969b5b5244"
+, sha256 ? "0dvl990alr4bb64w9b32dhzacvchpsspj8p3zqcgk7q5akvqh1mw"
+, pkgs   ? import (builtins.fetchTarball {
+    url = "https://github.com/NixOS/nixpkgs/archive/${rev}.tar.gz";
+    inherit sha256; }) {
+    config.allowUnfree = true;
+    config.allowBroken = false;
+  }
+}:
+
+let
+
+coq-haskell = coqPackages:
+  with pkgs.${coqPackages}; pkgs.stdenv.mkDerivation rec {
+    name = "coq${coq.coq-version}-coq-haskell-${version}";
+    version = "1.0";
+
+    src = pkgs.fetchFromGitHub {
+      owner  = "jwiegley";
+      repo   = "coq-haskell";
+      rev    = "08959da061eca867a3b09254960378d0450c501e";
+      sha256 = "1ydd4708hzhn2vf8xlx8axc1pmm386ll0mvi94n7sgfxb90lz1pc";
+    };
+
+    buildInputs = [
+      coq coq.ocaml coq.camlp5 coq.findlib pkgs.perl
+    ];
+    enableParallelBuilding = true;
+
+    buildFlags = [
+      "JOBS=$(NIX_BUILD_CORES)"
+    ];
+
+    installFlags = "COQLIB=$(out)/lib/coq/${coq.coq-version}/";
+
+    env = pkgs.buildEnv { inherit name; paths = buildInputs; };
+    passthru = {
+      compatibleCoqVersions = v: builtins.elem v [ "8.10" "8.11" "8.12" "8.13" "8.14" "8.15" ];
+    };
+  };
+
+linearscan = coqPackages:
+  with pkgs.${coqPackages}; pkgs.stdenv.mkDerivation rec {
+    name = "coq${coq.coq-version}-linearscan-${version}";
+    version = "1.0";
+
+    src = if pkgs ? coqFilterSource
+          then pkgs.coqFilterSource [] ./.
+          else ./.;
+
+    buildInputs = [
+      coq coq.ocaml coq.camlp5 coq.findlib mathcomp (coq-haskell coqPackages)
+    ];
+    enableParallelBuilding = true;
+
+    buildFlags = [
+      "JOBS=$(NIX_BUILD_CORES)"
+    ];
+
+    installFlags = "COQLIB=$(out)/lib/coq/${coq.coq-version}/";
+
+    env = pkgs.buildEnv { inherit name; paths = buildInputs; };
+    passthru = {
+      compatibleCoqVersions = v: builtins.elem v [ "8.10" "8.11" "8.12" "8.13" "8.14" "8.15" ];
+    };
+  };
+
+in {
+  linearscan_8_10 = linearscan "coqPackages_8_10";
+  linearscan_8_11 = linearscan "coqPackages_8_11";
+  linearscan_8_12 = linearscan "coqPackages_8_12";
+  linearscan_8_13 = linearscan "coqPackages_8_13";
+  linearscan_8_14 = linearscan "coqPackages_8_14";
+  linearscan_8_15 = linearscan "coqPackages_8_15";
+}
