shell.nix
@@ -1,0 +1,2 @@
+{ version ? "linearscan_8_15" }:
+(import ./default.nix {}).${version}
